new theory about code generation

Weidenbach_Book/CDCL_Two_Watched_Literals_List_Simple_Code.thy
@@ -1,77 +1,12 @@
 theory CDCL_Two_Watched_Literals_List_Simple_Code
   imports CDCL_Two_Watched_Literals_List DPLL_CDCL_W_Implementation
-    CDCL_Two_Watched_Literals_Initialisation
+    CDCL_Two_Watched_Literals_Initialisation CDCL_Two_Watched_Literals_Code_Common
 begin
 
 section \<open>CDCL Code (without caching clause watched by a literal)\<close>
-text \<open>
-  First we instantiate our types with sort heap, to show compatibility with code generation. The
-  idea is simplify to create injections into the components of our datatypes. This wirks since we
-  are not recursing through steps.
-\<close>
-instance literal :: (heap) heap
-proof standard
-  obtain f :: \<open>'a \<Rightarrow> nat\<close> where f: \<open>inj f\<close>
-    by blast
-  then have Hf: \<open>f x = f s \<longleftrightarrow> x = s\<close> for s x
-    unfolding inj_on_def Ball_def comp_def by blast
-  let ?f = \<open>\<lambda>L. (is_pos L, f (atm_of L))\<close>
-  have \<open>OFCLASS(bool \<times> nat, heap_class)\<close>
-   by standard
-  then obtain g :: \<open>bool \<times> nat \<Rightarrow> nat\<close> where g: \<open>inj g\<close>
-    by blast
-  then have H: \<open>g (x, y) = g (s, t) \<longleftrightarrow> x = s \<and> y = t\<close> for s t x y
-    unfolding inj_on_def Ball_def comp_def by blast
-  have \<open>inj (g o ?f)\<close>
-    using f g unfolding inj_on_def Ball_def comp_def H Hf
-    apply (intro allI impI)
-    apply (rename_tac x y, case_tac x; case_tac y)
-    by auto
-  then show \<open>\<exists>to_nat:: 'a literal \<Rightarrow> nat. inj to_nat\<close>
-    by blast
-qed
-
-instance annotated_lit :: (heap, heap, heap) heap
-proof standard
-  let ?f = \<open>\<lambda>L:: ('a, 'b, 'c) annotated_lit.
-      (if is_decided L then Some (lit_dec L) else None,
-       if is_decided L then None else Some (lit_prop L), if is_decided L then None else Some (mark_of L))\<close>
-    term ?f
-  have f: \<open>inj ?f\<close>
-    unfolding inj_on_def Ball_def
-    apply (intro allI impI)
-    apply (rename_tac x y, case_tac x; case_tac y)
-    by auto
-  then have Hf: \<open>?f x = ?f s \<longleftrightarrow> x = s\<close> for s x
-    unfolding inj_on_def Ball_def comp_def by blast
-  have \<open>OFCLASS('a option \<times> 'b option \<times> 'c option, heap_class)\<close>
-   by standard
-  then obtain g :: \<open>'a option \<times> 'b option \<times> 'c option \<Rightarrow> nat\<close> where g: \<open>inj g\<close>
-    by blast
-  then have H: \<open>g (x, y) = g (s, t) \<longleftrightarrow> x = s \<and> y = t\<close> for s t x y
-    unfolding inj_on_def Ball_def comp_def by blast
-  have \<open>inj (g o ?f)\<close>
-    using f g unfolding inj_on_def Ball_def comp_def H Hf
-    apply (intro allI impI)
-    apply (rename_tac x y, case_tac x; case_tac y)
-    by auto
-  then show \<open>\<exists>to_nat:: ('a, 'b, 'c) annotated_lit \<Rightarrow> nat. inj to_nat\<close>
-    by blast
-qed
-
 
 text \<open>Some functions and types:\<close>
-abbreviation nat_lit_assn :: "nat literal \<Rightarrow> nat literal \<Rightarrow> assn" where
-  \<open>nat_lit_assn \<equiv> (id_assn :: nat literal \<Rightarrow> _)\<close>
 
-abbreviation nat_ann_lit_assn :: "(nat, nat) ann_lit \<Rightarrow> (nat, nat) ann_lit \<Rightarrow> assn" where
-  \<open>nat_ann_lit_assn \<equiv> (id_assn :: (nat, nat) ann_lit \<Rightarrow> _)\<close>
-
-
-type_synonym ann_lits_l = \<open>(nat, nat) ann_lits\<close>
- 
-abbreviation nat_ann_lits_assn :: "ann_lits_l \<Rightarrow> ann_lits_l \<Rightarrow> assn" where
-  \<open>nat_ann_lits_assn \<equiv> list_assn nat_ann_lit_assn\<close>
 
 abbreviation nat_lits_trail_assn :: "ann_lits_l \<Rightarrow> (nat, nat) ann_lits \<Rightarrow> assn" where
   \<open>nat_lits_trail_assn \<equiv> list_assn (nat_ann_lit_assn :: (nat, nat) ann_lit \<Rightarrow> _)\<close>
@@ -115,189 +50,6 @@ abbreviation twl_st_l_assn :: \<open>nat twl_st_l \<Rightarrow> twl_st_ll \<Righ
  working_queue_l_assn *assn
  clause_l_assn
 \<close>
-
-subsection \<open>Declaration of some Operators and Implementation\<close>
-
-sepref_decl_op nat_lit_eq: "op = :: nat literal \<Rightarrow> nat literal \<Rightarrow> bool" ::
-  "(Id :: (nat literal \<times> _) set) \<rightarrow> (Id :: (nat literal \<times> _) set) \<rightarrow> (Id :: (bool \<times> _) set)" .
-
-lemma [def_pat_rules]:
-  "op = $ a $ b \<equiv> op_nat_lit_eq $ a $ b"
-  by auto
-
-term id_assn
-
-definition nat_ann_lit_eq_cases :: "(nat, nat) ann_lit \<Rightarrow> (nat, nat) ann_lit \<Rightarrow> bool" where
-  \<open>nat_ann_lit_eq_cases K L =
-    (case (K, L) of
-      (Decided K, Decided L) \<Rightarrow> K = L
-    | (Propagated K C, Propagated L C') \<Rightarrow> K = L \<and> C = C'
-    | (_, _) \<Rightarrow> False)\<close>
-
-definition nat_lit_eq_cases :: "nat literal \<Rightarrow> nat literal \<Rightarrow> bool" where
-  \<open>nat_lit_eq_cases K L =
-    (case (K, L) of
-      (Pos K, Pos L) \<Rightarrow> K = L
-    | (Neg K, Neg L) \<Rightarrow> K = L
-    | (_, _) \<Rightarrow> False)\<close>
-
-
-sepref_decl_op atm_of: "atm_of :: nat literal \<Rightarrow> nat" ::
-  "(Id :: (nat literal \<times> _) set) \<rightarrow> (Id :: (nat \<times> _) set)" .
-
-lemma [def_pat_rules]:
-  "atm_of \<equiv> op_atm_of"
-  by auto
-
-definition atm_of_impl  :: "nat literal \<Rightarrow> nat" where
-  \<open>atm_of_impl L = do {
-    case L of
-      Pos K \<Rightarrow> K
-    | Neg K \<Rightarrow> K}\<close>
-
-
-sepref_decl_op lit_of: "lit_of :: (nat, nat) ann_lit \<Rightarrow> nat literal" ::
-  "(Id :: ((nat, nat) ann_lit \<times> _) set) \<rightarrow> (Id :: (nat literal \<times> _) set)" .
-
-lemma [def_pat_rules]:
-  "lit_of \<equiv> op_lit_of"
-  by auto
-
-sepref_decl_op option_bool_eq: "op = :: bool option \<Rightarrow> bool option \<Rightarrow> bool" ::
-  "(Id :: ((bool option \<times> _) set)) \<rightarrow> (Id :: (bool option \<times> _) set) \<rightarrow> (Id :: (bool \<times> _) set)" .
-
-lemma [def_pat_rules]:
-  "op = $ a $ b \<equiv> op_option_bool_eq $ a $ b"
-  by auto
-
-sepref_decl_op case_bool: "case_bool :: 'a \<Rightarrow> 'a \<Rightarrow> bool \<Rightarrow> 'a" ::
-  "(Id :: (('a \<times> 'a) set)) \<rightarrow> (Id :: ('a \<times> 'a) set) \<rightarrow> (Id :: (bool \<times> _) set) \<rightarrow> (Id :: ('a \<times> 'a) set)" .
-
-
-lemma [def_pat_rules]:
-  "case_bool $ a $ b $ v \<equiv> op_case_bool $ a $ b $ v"
-  by auto
-
-definition option_bool_eq_impl :: \<open>bool option \<Rightarrow> bool option \<Rightarrow> bool\<close> where
-  \<open>option_bool_eq_impl L L' =
-   (if is_None L
-   then
-     if is_None L' then True else False
-   else
-    (if is_None L' then False else the L = the L'))\<close>
-
-definition lit_of_impl :: "(nat, nat) ann_lit \<Rightarrow> nat literal" where
-  \<open>lit_of_impl L = do {
-    case L of
-      Propagated K _ \<Rightarrow> K
-    | Decided K \<Rightarrow> K}\<close>
-
-
-definition case_bool_impl :: \<open>bool \<Rightarrow> bool \<Rightarrow> bool \<Rightarrow> bool\<close> where
-  \<open>case_bool_impl L L' v = do {if v then L else L'}\<close>
-
-context
-  notes [intro!] = hfrefI hn_refineI[THEN hn_refine_preI] frefI
-  notes [simp] = pure_def hn_ctxt_def invalid_assn_def
-begin
-
-lemma nat_lit_eq_cases_refine[sepref_fr_rules]:
-  \<open>(uncurry (return oo nat_lit_eq_cases), uncurry (RETURN oo op_nat_lit_eq)) \<in>
-    nat_lit_assn\<^sup>k *\<^sub>a nat_lit_assn\<^sup>k \<rightarrow>\<^sub>a bool_assn\<close>
-  unfolding nat_lit_eq_cases_def
-  apply (sep_auto split: literal.split)
-  apply (rename_tac aa ba a b)
-  apply (case_tac aa; case_tac ba; sep_auto)
-  done
-
-sepref_decl_impl nat_lit_eq_cases: nat_lit_eq_cases_refine .
-
-
-lemma atom_of_impl_refine[sepref_fr_rules]:
-  \<open>(return o atm_of_impl, RETURN o op_atm_of) \<in> nat_lit_assn\<^sup>k \<rightarrow>\<^sub>a nat_assn\<close>
-  unfolding op_atm_of_def atm_of_impl_def
-  by (sep_auto split: literal.split)
-
-sepref_decl_impl atom_of_impl: atom_of_impl_refine .
-
-lemma lit_of_impl_refine[sepref_fr_rules]:
-  \<open>(return o lit_of_impl, RETURN o op_lit_of) \<in> nat_ann_lit_assn\<^sup>k \<rightarrow>\<^sub>a nat_lit_assn\<close>
-  unfolding op_lit_of_def lit_of_impl_def
-  by (sep_auto split: annotated_lit.splits)
-
-sepref_decl_impl lit_of_impl: atom_of_impl_refine .
-
-lemma option_bool_eq_impl_option_op_bool_eq_impl: \<open>option_bool_eq_impl = op_option_bool_eq\<close>
-  unfolding option_bool_eq_impl_def op_option_bool_eq_def by (auto split: option.splits intro!: ext)
-
-lemma option_bool_eq_refine[sepref_fr_rules]:
-  \<open>(uncurry (return oo option_bool_eq_impl), uncurry (RETURN oo op_option_bool_eq)) \<in>
-    (option_assn bool_assn)\<^sup>k *\<^sub>a (option_assn bool_assn)\<^sup>k \<rightarrow>\<^sub>a bool_assn\<close>
-  unfolding option_bool_eq_impl_option_op_bool_eq_impl
-  unfolding op_option_bool_eq_def
-  apply sep_auto
-  subgoal for b aa ba ab bb ac bc by (cases b; cases ba; cases aa; auto)
-  subgoal for b aa ba ab bb ac bc by (cases b; cases ba; cases aa; auto)
-  done
-
-sepref_decl_impl option_bool_eq: option_bool_eq_refine .
-
-lemma case_bool_impl_refine[sepref_fr_rules]:
-  \<open>(uncurry2 (return ooo (case_bool_impl :: bool \<Rightarrow> bool \<Rightarrow> bool \<Rightarrow> bool)),
-       uncurry2 (RETURN ooo op_case_bool)) \<in>
-    (id_assn :: bool \<Rightarrow> _)\<^sup>k *\<^sub>a (id_assn :: bool \<Rightarrow> _)\<^sup>k *\<^sub>a (bool_assn)\<^sup>k \<rightarrow>\<^sub>a id_assn\<close>
-  unfolding case_bool_impl_def
-  unfolding op_option_bool_eq_def
-  apply (sep_auto split!: if_splits option.splits)
-  apply (case_tac bc)
-  apply auto
-  done
-
-sepref_decl_impl case_bool: case_bool_impl_refine .
-
-end
-
-sepref_decl_op defined_lit_imp: "defined_lit:: (nat, nat) ann_lit list \<Rightarrow> nat literal \<Rightarrow> bool" ::
-  "(Id :: ((nat, nat) ann_lit list \<times> _) set) \<rightarrow> (Id :: (nat literal \<times> _) set) \<rightarrow> bool_rel" .
-
-lemma [def_pat_rules]:
-  "defined_lit $ a $ b \<equiv> op_defined_lit_imp $ a $ b"
-  by auto
-
-definition defined_lit_set :: \<open>('a, 'm) ann_lit set \<Rightarrow> 'a literal \<Rightarrow> bool\<close>
-  where
-\<open>defined_lit_set I L \<longleftrightarrow> (Decided L \<in> I) \<or> (\<exists>P. Propagated L P \<in>  I)
-  \<or> (Decided (-L) \<in> I) \<or> (\<exists>P. Propagated (-L) P \<in>  I)\<close>
-
-lemma defined_lit_defined_lit_set: \<open>defined_lit M L \<longleftrightarrow> defined_lit_set (set M) L\<close>
-  unfolding defined_lit_set_def defined_lit_def
-  by auto
-
-lemma defined_lit_set_insert: \<open>defined_lit_set (insert L' M) L \<longleftrightarrow> atm_of (lit_of L') = atm_of L \<or> defined_lit_set M L\<close>
-  unfolding defined_lit_set_def
-  by (cases L') (auto dest!: literal_is_lit_of_decided simp: atm_of_eq_atm_of)
-
-lemma defined_lit_set_nil[simp]: \<open>\<not>defined_lit_set {} L\<close>
-   unfolding defined_lit_set_def by auto
-
-lemma defined_lit_set_mono: \<open>M \<subseteq> M' \<Longrightarrow> defined_lit_set M L \<Longrightarrow> defined_lit_set M' L\<close>
-   unfolding defined_lit_set_def by auto
-
-definition defined_lit_map_impl :: "(nat, nat) ann_lit list \<Rightarrow> nat literal \<Rightarrow> bool nres" where
-  \<open>defined_lit_map_impl M L =
-  nfoldli M
-     (\<lambda>brk. brk = False)
-     (\<lambda>L' _. do {
-       let L\<^sub>1 = atm_of L;
-       let L\<^sub>1'' = atm_of (lit_of L');
-       RETURN (L\<^sub>1 = L\<^sub>1'')})
-    False\<close>
-
-sepref_definition defined_lit_map_impl' is
-  \<open>uncurry (defined_lit_map_impl :: (nat, nat) ann_lit list \<Rightarrow> _)\<close> ::
-  \<open>(nat_ann_lits_assn)\<^sup>k *\<^sub>a nat_lit_assn\<^sup>k \<rightarrow>\<^sub>a bool_assn\<close>
-  unfolding defined_lit_map_impl_def
-  by sepref
 
 lemma defined_lit_map_impl_denifend_lit: \<open>defined_lit_map_impl M L \<le> SPEC (op = (defined_lit M L))\<close>
   unfolding defined_lit_map_impl_def
@@ -361,32 +113,11 @@ definition valued'  :: "(nat, nat) ann_lits \<Rightarrow> nat literal \<Rightarr
   \<open>valued' = valued\<close>
 
 
-(* lemma [sepref_import_param]:
-  \<open>(uncurry (RETURN oo valued), uncurry (RETURN oo valued)) \<in> Id \<rightarrow> \<langle>Id\<rangle>nres_rel\<close>
-  by (auto simp: nres_rel_def) *)
-
-(* sepref_register \<open>valued' :: ((nat, nat) ann_lits \<Rightarrow> nat literal \<Rightarrow> bool option)\<close>
-
-lemma valued_impl'_refine[sepref_fr_rules]:
-  shows \<open>(uncurry valued_impl', uncurry (RETURN oo valued)) \<in>
-    [\<lambda>(M, _). no_dup M]\<^sub>a (nat_ann_lits_assn)\<^sup>k *\<^sub>a nat_lit_assn\<^sup>k \<rightarrow> option_assn bool_assn\<close>
-  using valued_impl'.refine_raw[unfolded valued_impl'_def[symmetric], FCOMP valued_impl_spec]
-  unfolding hrp_comp_Id2 valued'_def .
-
-concrete_definition valued'_impl_impl uses valued_impl'_refine
- *)
 context
   notes [intro!] = hfrefI hn_refineI[THEN hn_refine_preI] frefI
   notes [simp] = pure_def hn_ctxt_def invalid_assn_def
 begin
 
-(*
-
-lemma [sepref_import_param]:
-  \<open>(uncurry (RETURN oo valued), uncurry (RETURN oo valued)) \<in> Id \<rightarrow> \<langle>Id\<rangle>nres_rel\<close>
-  by (auto simp: nres_rel_def)
- *)
-(* sepref_register \<open>valued' :: ((nat, nat) ann_lits \<Rightarrow> nat literal \<Rightarrow> bool option)\<close> *)
 sepref_decl_op valued: \<open>valued :: ((nat, nat) ann_lits \<Rightarrow> nat literal \<Rightarrow> bool option)\<close>
   :: "(Id :: ((nat, nat) ann_lits \<times>_)set) \<rightarrow> (Id :: (nat literal \<times> _) set) \<rightarrow> (Id :: (bool option\<times> _) set)"
   .
@@ -409,36 +140,12 @@ sepref_decl_impl valued: valued_impl'_refine
   by simp
 
 end
-term find_unwatched_impl
-(* concrete_definition valued'_impl_impl uses valued_impl'_refine *)
 
-(*
-lemma [safe_constraint_rules]: \<open>is_pure R \<Longrightarrow> is_pure (nat_ann_lits_assn R)\<close>
-  by (simp add: list_assn_pure_conv) *)
-(* definition find_unwatched :: "('a, 'b) ann_lits \<Rightarrow> 'a clause_l \<Rightarrow> (bool option \<times> nat) nres" where
-\<open>find_unwatched M C = do {
-  WHILE\<^sub>T\<^bsup>\<lambda>(found, i). i \<ge> 2 \<and> i \<le> length C \<and> (\<forall>j\<in>{2..<i}. -(C!j) \<in> lits_of_l M) \<and>
-    (found = Some False \<longrightarrow> (undefined_lit M (C!i) \<and> i < length C)) \<and>
-    (found = Some True \<longrightarrow> (C!i \<in> lits_of_l M \<and> i < length C)) \<^esup>
-    (\<lambda>(found, i). found = None \<and> i < length C)
-    (\<lambda>(_, i). do {
-      ASSERT(i < length C);
-      case valued M (C!i) of
-        None \<Rightarrow> do { RETURN (Some False, i)}
-      | Some v \<Rightarrow>
-         (if v then do { RETURN (Some True, i)} else do { RETURN (None, i+1)})
-      }
-    )
-    (None, 2::nat)
-  }
-\<close> *)
-
-term find_unwatched
 sepref_definition find_unwatched_impl is
    "uncurry (find_unwatched :: (nat, nat) ann_lits
       \<Rightarrow> nat literal list \<Rightarrow> (bool option \<times> nat) nres)"
   :: \<open>[\<lambda>(M, L). no_dup M]\<^sub>anat_ann_lits_assn\<^sup>k *\<^sub>a (list_assn nat_lit_assn)\<^sup>k \<rightarrow> prod_assn (option_assn bool_assn) nat_assn\<close>
-  unfolding find_unwatched_def (* valued'_def[symmetric] *)
+  unfolding find_unwatched_def
   supply [[goals_limit=1]]
   by sepref
 
@@ -503,9 +210,11 @@ lemma [sepref_fr_rules]:
       intro: Assertions.mod_emp_simp)
   done
 
+
 subsection \<open>Code Generation\<close>
 
 subsubsection \<open>The Body of the Inner Propagation\<close>
+
 sepref_definition unit_propagation_inner_loop_body_l_impl is \<open>uncurry2 (unit_propagation_inner_loop_body_l :: nat literal \<Rightarrow> nat \<Rightarrow>
   nat twl_st_l \<Rightarrow> nat twl_st_l nres)\<close> ::
   \<open>nat_lit_assn\<^sup>k *\<^sub>a nat_assn\<^sup>k *\<^sub>a twl_st_l_assn\<^sup>d \<rightarrow>\<^sub>a twl_st_l_assn\<close>
@@ -1672,7 +1381,7 @@ thm cdcl_twl_stgy_prog_l_impl_spec_final[unfolded full_cdcl_twl_stgy_def]
 export_code cdcl_twl_stgy_prog_l_impl in SML_imp module_name CDCL_Non_Cached_List
   file "code/CDCL_Non_Cached_List.ML"
 
-    
+
 section \<open>Code for the initialisation of the Data Structure\<close>
 
 definition init_dt_step_l :: \<open>'v clause_l \<Rightarrow> 'v twl_st_l \<Rightarrow> ('v twl_st_l) nres\<close> where
