Weidenbach_Book/CDCL_Two_Watched_Literals_Code_Common.thy
@@ -1,0 +1,256 @@
+theory CDCL_Two_Watched_Literals_Code_Common
+  imports "Partial_Annotated_Clausal_Logic" IICF
+begin
+text \<open>
+  First we instantiate our types with sort heap, to show compatibility with code generation. The
+  idea is simplify to create injections into the components of our datatypes. This wirks since we
+  are not recursing through steps.
+\<close>
+instance literal :: (heap) heap
+proof standard
+  obtain f :: \<open>'a \<Rightarrow> nat\<close> where f: \<open>inj f\<close>
+    by blast
+  then have Hf: \<open>f x = f s \<longleftrightarrow> x = s\<close> for s x
+    unfolding inj_on_def Ball_def comp_def by blast
+  let ?f = \<open>\<lambda>L. (is_pos L, f (atm_of L))\<close>
+  have \<open>OFCLASS(bool \<times> nat, heap_class)\<close>
+   by standard
+  then obtain g :: \<open>bool \<times> nat \<Rightarrow> nat\<close> where g: \<open>inj g\<close>
+    by blast
+  then have H: \<open>g (x, y) = g (s, t) \<longleftrightarrow> x = s \<and> y = t\<close> for s t x y
+    unfolding inj_on_def Ball_def comp_def by blast
+  have \<open>inj (g o ?f)\<close>
+    using f g unfolding inj_on_def Ball_def comp_def H Hf
+    apply (intro allI impI)
+    apply (rename_tac x y, case_tac x; case_tac y)
+    by auto
+  then show \<open>\<exists>to_nat:: 'a literal \<Rightarrow> nat. inj to_nat\<close>
+    by blast
+qed
+
+instance annotated_lit :: (heap, heap, heap) heap
+proof standard
+  let ?f = \<open>\<lambda>L:: ('a, 'b, 'c) annotated_lit.
+      (if is_decided L then Some (lit_dec L) else None,
+       if is_decided L then None else Some (lit_prop L), if is_decided L then None else Some (mark_of L))\<close>
+    term ?f
+  have f: \<open>inj ?f\<close>
+    unfolding inj_on_def Ball_def
+    apply (intro allI impI)
+    apply (rename_tac x y, case_tac x; case_tac y)
+    by auto
+  then have Hf: \<open>?f x = ?f s \<longleftrightarrow> x = s\<close> for s x
+    unfolding inj_on_def Ball_def comp_def by blast
+  have \<open>OFCLASS('a option \<times> 'b option \<times> 'c option, heap_class)\<close>
+   by standard
+  then obtain g :: \<open>'a option \<times> 'b option \<times> 'c option \<Rightarrow> nat\<close> where g: \<open>inj g\<close>
+    by blast
+  then have H: \<open>g (x, y) = g (s, t) \<longleftrightarrow> x = s \<and> y = t\<close> for s t x y
+    unfolding inj_on_def Ball_def comp_def by blast
+  have \<open>inj (g o ?f)\<close>
+    using f g unfolding inj_on_def Ball_def comp_def H Hf
+    apply (intro allI impI)
+    apply (rename_tac x y, case_tac x; case_tac y)
+    by auto
+  then show \<open>\<exists>to_nat:: ('a, 'b, 'c) annotated_lit \<Rightarrow> nat. inj to_nat\<close>
+    by blast
+qed
+
+
+subsection \<open>Declaration of some Operators and Implementation\<close>
+
+sepref_decl_op nat_lit_eq: "op = :: nat literal \<Rightarrow> nat literal \<Rightarrow> bool" ::
+  "(Id :: (nat literal \<times> _) set) \<rightarrow> (Id :: (nat literal \<times> _) set) \<rightarrow> (Id :: (bool \<times> _) set)" .
+
+lemma [def_pat_rules]:
+  "op = $ a $ b \<equiv> op_nat_lit_eq $ a $ b"
+  by auto
+
+term id_assn
+
+definition nat_ann_lit_eq_cases :: "(nat, nat) ann_lit \<Rightarrow> (nat, nat) ann_lit \<Rightarrow> bool" where
+  \<open>nat_ann_lit_eq_cases K L =
+    (case (K, L) of
+      (Decided K, Decided L) \<Rightarrow> K = L
+    | (Propagated K C, Propagated L C') \<Rightarrow> K = L \<and> C = C'
+    | (_, _) \<Rightarrow> False)\<close>
+
+definition nat_lit_eq_cases :: "nat literal \<Rightarrow> nat literal \<Rightarrow> bool" where
+  \<open>nat_lit_eq_cases K L =
+    (case (K, L) of
+      (Pos K, Pos L) \<Rightarrow> K = L
+    | (Neg K, Neg L) \<Rightarrow> K = L
+    | (_, _) \<Rightarrow> False)\<close>
+
+
+sepref_decl_op atm_of: "atm_of :: nat literal \<Rightarrow> nat" ::
+  "(Id :: (nat literal \<times> _) set) \<rightarrow> (Id :: (nat \<times> _) set)" .
+
+lemma [def_pat_rules]:
+  "atm_of \<equiv> op_atm_of"
+  by auto
+
+definition atm_of_impl  :: "nat literal \<Rightarrow> nat" where
+  \<open>atm_of_impl L = do {
+    case L of
+      Pos K \<Rightarrow> K
+    | Neg K \<Rightarrow> K}\<close>
+
+
+sepref_decl_op lit_of: "lit_of :: (nat, nat) ann_lit \<Rightarrow> nat literal" ::
+  "(Id :: ((nat, nat) ann_lit \<times> _) set) \<rightarrow> (Id :: (nat literal \<times> _) set)" .
+
+lemma [def_pat_rules]:
+  "lit_of \<equiv> op_lit_of"
+  by auto
+
+sepref_decl_op option_bool_eq: "op = :: bool option \<Rightarrow> bool option \<Rightarrow> bool" ::
+  "(Id :: ((bool option \<times> _) set)) \<rightarrow> (Id :: (bool option \<times> _) set) \<rightarrow> (Id :: (bool \<times> _) set)" .
+
+lemma [def_pat_rules]:
+  "op = $ a $ b \<equiv> op_option_bool_eq $ a $ b"
+  by auto
+
+sepref_decl_op case_bool: "case_bool :: 'a \<Rightarrow> 'a \<Rightarrow> bool \<Rightarrow> 'a" ::
+  "(Id :: (('a \<times> 'a) set)) \<rightarrow> (Id :: ('a \<times> 'a) set) \<rightarrow> (Id :: (bool \<times> _) set) \<rightarrow> (Id :: ('a \<times> 'a) set)" .
+
+
+lemma [def_pat_rules]:
+  "case_bool $ a $ b $ v \<equiv> op_case_bool $ a $ b $ v"
+  by auto
+
+definition option_bool_eq_impl :: \<open>bool option \<Rightarrow> bool option \<Rightarrow> bool\<close> where
+  \<open>option_bool_eq_impl L L' =
+   (if is_None L
+   then
+     if is_None L' then True else False
+   else
+    (if is_None L' then False else the L = the L'))\<close>
+
+definition lit_of_impl :: "(nat, nat) ann_lit \<Rightarrow> nat literal" where
+  \<open>lit_of_impl L = do {
+    case L of
+      Propagated K _ \<Rightarrow> K
+    | Decided K \<Rightarrow> K}\<close>
+
+
+definition case_bool_impl :: \<open>bool \<Rightarrow> bool \<Rightarrow> bool \<Rightarrow> bool\<close> where
+  \<open>case_bool_impl L L' v = do {if v then L else L'}\<close>
+
+
+text \<open>Some functions and types:\<close>
+abbreviation nat_lit_assn :: "nat literal \<Rightarrow> nat literal \<Rightarrow> assn" where
+  \<open>nat_lit_assn \<equiv> (id_assn :: nat literal \<Rightarrow> _)\<close>
+
+abbreviation nat_ann_lit_assn :: "(nat, nat) ann_lit \<Rightarrow> (nat, nat) ann_lit \<Rightarrow> assn" where
+  \<open>nat_ann_lit_assn \<equiv> (id_assn :: (nat, nat) ann_lit \<Rightarrow> _)\<close>
+
+type_synonym ann_lits_l = \<open>(nat, nat) ann_lits\<close>
+
+abbreviation nat_ann_lits_assn :: "ann_lits_l \<Rightarrow> ann_lits_l \<Rightarrow> assn" where
+  \<open>nat_ann_lits_assn \<equiv> list_assn nat_ann_lit_assn\<close>
+
+context
+  notes [intro!] = hfrefI hn_refineI[THEN hn_refine_preI] frefI
+  notes [simp] = pure_def hn_ctxt_def invalid_assn_def
+begin
+
+lemma nat_lit_eq_cases_refine[sepref_fr_rules]:
+  \<open>(uncurry (return oo nat_lit_eq_cases), uncurry (RETURN oo op_nat_lit_eq)) \<in>
+    nat_lit_assn\<^sup>k *\<^sub>a nat_lit_assn\<^sup>k \<rightarrow>\<^sub>a bool_assn\<close>
+  unfolding nat_lit_eq_cases_def
+  apply (sep_auto split: literal.split)
+  apply (rename_tac aa ba a b)
+  apply (case_tac aa; case_tac ba; sep_auto)
+  done
+
+sepref_decl_impl nat_lit_eq_cases: nat_lit_eq_cases_refine .
+
+
+lemma atom_of_impl_refine[sepref_fr_rules]:
+  \<open>(return o atm_of_impl, RETURN o op_atm_of) \<in> nat_lit_assn\<^sup>k \<rightarrow>\<^sub>a nat_assn\<close>
+  unfolding op_atm_of_def atm_of_impl_def
+  by (sep_auto split: literal.split)
+
+sepref_decl_impl atom_of_impl: atom_of_impl_refine .
+
+lemma lit_of_impl_refine[sepref_fr_rules]:
+  \<open>(return o lit_of_impl, RETURN o op_lit_of) \<in> nat_ann_lit_assn\<^sup>k \<rightarrow>\<^sub>a nat_lit_assn\<close>
+  unfolding op_lit_of_def lit_of_impl_def
+  by (sep_auto split: annotated_lit.splits)
+
+sepref_decl_impl lit_of_impl: atom_of_impl_refine .
+
+lemma option_bool_eq_impl_option_op_bool_eq_impl: \<open>option_bool_eq_impl = op_option_bool_eq\<close>
+  unfolding option_bool_eq_impl_def op_option_bool_eq_def by (auto split: option.splits intro!: ext)
+
+lemma option_bool_eq_refine[sepref_fr_rules]:
+  \<open>(uncurry (return oo option_bool_eq_impl), uncurry (RETURN oo op_option_bool_eq)) \<in>
+    (option_assn bool_assn)\<^sup>k *\<^sub>a (option_assn bool_assn)\<^sup>k \<rightarrow>\<^sub>a bool_assn\<close>
+  unfolding option_bool_eq_impl_option_op_bool_eq_impl
+  unfolding op_option_bool_eq_def
+  apply sep_auto
+  subgoal for b aa ba ab bb ac bc by (cases b; cases ba; cases aa; auto)
+  subgoal for b aa ba ab bb ac bc by (cases b; cases ba; cases aa; auto)
+  done
+
+sepref_decl_impl option_bool_eq: option_bool_eq_refine .
+
+lemma case_bool_impl_refine[sepref_fr_rules]:
+  \<open>(uncurry2 (return ooo (case_bool_impl :: bool \<Rightarrow> bool \<Rightarrow> bool \<Rightarrow> bool)),
+       uncurry2 (RETURN ooo op_case_bool)) \<in>
+    (id_assn :: bool \<Rightarrow> _)\<^sup>k *\<^sub>a (id_assn :: bool \<Rightarrow> _)\<^sup>k *\<^sub>a (bool_assn)\<^sup>k \<rightarrow>\<^sub>a id_assn\<close>
+  unfolding case_bool_impl_def
+  unfolding op_option_bool_eq_def
+  apply (sep_auto split!: if_splits option.splits)
+  apply (case_tac bc)
+  apply auto
+  done
+
+sepref_decl_impl case_bool: case_bool_impl_refine .
+
+end
+
+sepref_decl_op defined_lit_imp: "defined_lit:: (nat, nat) ann_lit list \<Rightarrow> nat literal \<Rightarrow> bool" ::
+  "(Id :: ((nat, nat) ann_lit list \<times> _) set) \<rightarrow> (Id :: (nat literal \<times> _) set) \<rightarrow> bool_rel" .
+
+lemma [def_pat_rules]:
+  "defined_lit $ a $ b \<equiv> op_defined_lit_imp $ a $ b"
+  by auto
+
+definition defined_lit_set :: \<open>('a, 'm) ann_lit set \<Rightarrow> 'a literal \<Rightarrow> bool\<close>
+  where
+\<open>defined_lit_set I L \<longleftrightarrow> (Decided L \<in> I) \<or> (\<exists>P. Propagated L P \<in>  I)
+  \<or> (Decided (-L) \<in> I) \<or> (\<exists>P. Propagated (-L) P \<in>  I)\<close>
+
+lemma defined_lit_defined_lit_set: \<open>defined_lit M L \<longleftrightarrow> defined_lit_set (set M) L\<close>
+  unfolding defined_lit_set_def defined_lit_def
+  by auto
+
+lemma defined_lit_set_insert: \<open>defined_lit_set (insert L' M) L \<longleftrightarrow> atm_of (lit_of L') = atm_of L \<or> defined_lit_set M L\<close>
+  unfolding defined_lit_set_def
+  by (cases L') (auto dest!: literal_is_lit_of_decided simp: atm_of_eq_atm_of)
+
+lemma defined_lit_set_nil[simp]: \<open>\<not>defined_lit_set {} L\<close>
+   unfolding defined_lit_set_def by auto
+
+lemma defined_lit_set_mono: \<open>M \<subseteq> M' \<Longrightarrow> defined_lit_set M L \<Longrightarrow> defined_lit_set M' L\<close>
+   unfolding defined_lit_set_def by auto
+
+definition defined_lit_map_impl :: "(nat, nat) ann_lit list \<Rightarrow> nat literal \<Rightarrow> bool nres" where
+  \<open>defined_lit_map_impl M L =
+  nfoldli M
+     (\<lambda>brk. brk = False)
+     (\<lambda>L' _. do {
+       let L\<^sub>1 = atm_of L;
+       let L\<^sub>1'' = atm_of (lit_of L');
+       RETURN (L\<^sub>1 = L\<^sub>1'')})
+    False\<close>
+
+sepref_definition defined_lit_map_impl' is
+  \<open>uncurry (defined_lit_map_impl :: (nat, nat) ann_lit list \<Rightarrow> _)\<close> ::
+  \<open>(nat_ann_lits_assn)\<^sup>k *\<^sub>a nat_lit_assn\<^sup>k \<rightarrow>\<^sub>a bool_assn\<close>
+  unfolding defined_lit_map_impl_def
+  by sepref
+
+end
