Weidenbach_Book/CDCL_Two_Watched_Literals_List_Watched_Code.thy
@@ -1,57 +1,7 @@
 theory CDCL_Two_Watched_Literals_List_Watched_Code
   imports CDCL_Two_Watched_Literals_List_Watched Array_Array_List
+    CDCL_Two_Watched_Literals_Code_Common
 begin
-
-instance literal :: (heap) heap
-proof standard
-  obtain f :: \<open>'a \<Rightarrow> nat\<close> where f: \<open>inj f\<close>
-    by blast
-  then have Hf: \<open>f x = f s \<longleftrightarrow> x = s\<close> for s x
-    unfolding inj_on_def Ball_def comp_def by blast
-  let ?f = \<open>\<lambda>L. (is_pos L, f (atm_of L))\<close>
-  have \<open>OFCLASS(bool \<times> nat, heap_class)\<close>
-   by standard
-  then obtain g :: \<open>bool \<times> nat \<Rightarrow> nat\<close> where g: \<open>inj g\<close>
-    by blast
-  then have H: \<open>g (x, y) = g (s, t) \<longleftrightarrow> x = s \<and> y = t\<close> for s t x y
-    unfolding inj_on_def Ball_def comp_def by blast
-  have \<open>inj (g o ?f)\<close>
-    using f g unfolding inj_on_def Ball_def comp_def H Hf
-    apply (intro allI impI)
-    apply (rename_tac x y, case_tac x; case_tac y)
-    by auto
-  then show \<open>\<exists>to_nat:: 'a literal \<Rightarrow> nat. inj to_nat\<close>
-    by blast
-qed
-
-instance annotated_lit :: (heap, heap, heap) heap
-proof standard
-  let ?f = \<open>\<lambda>L:: ('a, 'b, 'c) annotated_lit.
-      (if is_decided L then Some (lit_dec L) else None,
-       if is_decided L then None else Some (lit_prop L), if is_decided L then None else Some (mark_of L))\<close>
-    term ?f
-  have f: \<open>inj ?f\<close>
-    unfolding inj_on_def Ball_def
-    apply (intro allI impI)
-    apply (rename_tac x y, case_tac x; case_tac y)
-    by auto
-  then have Hf: \<open>?f x = ?f s \<longleftrightarrow> x = s\<close> for s x
-    unfolding inj_on_def Ball_def comp_def by blast
-  have \<open>OFCLASS('a option \<times> 'b option \<times> 'c option, heap_class)\<close>
-   by standard
-  then obtain g :: \<open>'a option \<times> 'b option \<times> 'c option \<Rightarrow> nat\<close> where g: \<open>inj g\<close>
-    by blast
-  then have H: \<open>g (x, y) = g (s, t) \<longleftrightarrow> x = s \<and> y = t\<close> for s t x y
-    unfolding inj_on_def Ball_def comp_def by blast
-  have \<open>inj (g o ?f)\<close>
-    using f g unfolding inj_on_def Ball_def comp_def H Hf
-    apply (intro allI impI)
-    apply (rename_tac x y, case_tac x; case_tac y)
-    by auto
-  then show \<open>\<exists>to_nat:: ('a, 'b, 'c) annotated_lit \<Rightarrow> nat. inj to_nat\<close>
-    by blast
-qed
-
 
 section \<open>Code Generation\<close>
 
